benchmark/benchmark.v
@@ -6,6 +6,9 @@ From stablesort Require Import stablesort.
 Elpi Command sort_benchmark.
 Elpi Accumulate lp:{{
 
+kind triple type -> type -> type -> type.
+type triple A -> B -> C -> triple A B C.
+
 % [positive-constant N T] states that [T] is a Coq term of type [positive]
 % corresponding to [N].
 pred positive-constant o:int, o:term.
@@ -60,55 +63,93 @@ median TS Out :-
   1 is {std.length TS} mod 2, !,
   std.nth {calc ({std.length TS} div 2)} {sort TS} Out.
 
-pred time-median-rec i:int, i:prop, i:list float, o:float.
-time-median-rec 0 _ TS Out :- !, median TS Out.
-time-median-rec N P TS Out :- !,
-  0 < N, !,
-  std.time P Time, !,
-  time-median-rec {calc (N - 1)} P [Time|TS] Out.
+pred time-median-rec
+  i:int, i:prop, i:list float, i:list float, o:float, o:float.
+time-median-rec 0 _ TS WS TOut WOut :- !, median TS TOut, median WS WOut.
+time-median-rec N P TS WS TOut WOut :- std.do! [
+  0 < N,
+  % invoke GC explicitly before each measurement
+  gc.compact,
+  % change the verbosity to observe automatic GC invocation
+  gc.get _ _ _ Verbose _ _ _ _,
+  gc.set _ _ _ 31 _ _ _ _,
+  % check for the amount of memory allocated
+  gc.quick-stat Minor1 Promoted1 Major1 _ _ _ _ _ _ _,
+  % measurement
+  std.time P Time,
+  % check for the amount of memory allocated, again
+  gc.quick-stat Minor2 Promoted2 Major2 _ _ _ _ _ _ _,
+  % restore the verbosity
+  gc.set _ _ _ Verbose _ _ _ _,
+  Words is ((Minor2 + Major2 - Promoted2) - (Minor1 + Major1 - Promoted1)),
+  time-median-rec {calc (N - 1)} P [Time|TS] [Words|WS] TOut WOut
+].
 
-pred time-median i:int, i:prop, o:float.
-time-median N P Out :- !, time-median-rec N P [] Out.
+pred time-median i:int, i:prop, o:float, o:float.
+time-median N P Time Words :- !, time-median-rec N P [] [] Time Words.
 
 %%%%%%%%%%%%%%%%%%%%%%%%%%%%%%%%%%%%%%%%%%%%%%%%%%%%%%%%%%%%%%%%%%%%%%%%%%%%%%%%
 
-pred benchmark-case i:string, i:(term -> term -> term -> prop),
-                    i:list (pair string term), i:int.
-benchmark-case RedStr Red Config Size :- std.do! [
+pred benchmark-case
+  i:string, i:(term -> term -> term -> prop),
+  i:list (pair string term), i:int, o:list string, o:list string.
+benchmark-case RedStr Red Config Size TS MS :- std.do! [
   coq.env.begin-section "Sec",
   random-N-list Size Size Input,
   ID is "input_" ^ { std.any->string {new_int} },
   @local! => coq.env.add-const ID Input {{ list N }} @transparent! C,
-  std.map Config (c\ r\ sigma Name Func Computation Time TimeStr\ std.do! [
-    c = pr Name Func,
-    Computation = {{ lp:Func N N.leb lp:{{ global (const C) }} }},
-    std.assert-ok! (coq.typecheck Computation {{ list N }}) "bad term",
-    time-median 5 (Red Computation {{ list N }} _) Time,
-    std.any->string Time TimeStr,
-    r is Name ^ ": " ^ TimeStr
-  ]) RS,
-  Str is RedStr ^ ", size: " ^ {std.any->string Size} ^ ", " ^
-         {std.string.concat ", " RS},
+  std.map Config
+    (c\ r\ sigma Name Func Comp CompTy Time Words Mem TStr MStr\ std.do! [
+      c = pr Name Func,
+      Comp = {{ lp:Func lp:{{ global (const C) }} }},
+      std.assert-ok! (coq.typecheck Comp CompTy) "bad term",
+      time-median 5 (Red Comp CompTy _) Time Words,
+      std.any->string Time TStr,
+      Mem is Words / (128.0 * 1024.0), % memory consumption in MBs
+      std.any->string Mem MStr,
+      r is triple Name TStr MStr
+    ]) RS,
+  std.any->string Size SizeStr,
+  Str is RedStr ^ ", size: " ^ SizeStr ^ "; " ^
+         {std.string.concat "; "
+            {std.map RS (r\ s\ sigma Name TStr MStr\
+               r = triple Name TStr MStr,
+               s is Name ^ ": " ^ TStr ^ "s, " ^ MStr ^ "MB")} },
   coq.say Str,
+  std.map RS (r\ s\ sigma Name TStr MStr\
+    r = triple Name TStr MStr,
+    s is "(" ^ SizeStr ^ ", " ^ TStr ^ ")"
+  ) TS,
+  std.map RS (r\ s\ sigma Name TStr MStr\
+    r = triple Name TStr MStr,
+    s is "(" ^ SizeStr ^ ", " ^ MStr ^ ")"
+  ) MS,
   coq.env.end-section
 ].
 
-pred benchmark i:string, i:(term -> term -> term -> prop),
-               i:list (pair string term), i:int, i:int, i:int.
-benchmark _ _ _ 0 _ _ :- !.
-benchmark RedStr Red Config Repeat Incr CurrentSize :- std.do! [
+pred benchmark
+  i:string, i:(term -> term -> term -> prop),
+  i:list (pair string term), i:int, i:int, i:int,
+  o:list (list string), o:list (list string).
+benchmark _ _ Config 0 _ _ SS SS :- !,
+  std.map Config (_\ r\ r = []) SS.
+benchmark RedStr Red Config Repeat Incr CurrentSize TSS' MSS' :- std.do! [
   0 < Repeat,
   NextSize is CurrentSize + Incr,
-  benchmark-case RedStr Red Config NextSize,
-  benchmark RedStr Red Config {calc (Repeat - 1)} Incr NextSize
+  benchmark-case RedStr Red Config NextSize TS MS,
+  benchmark RedStr Red Config {calc (Repeat - 1)} Incr NextSize TSS MSS,
+  std.map2 TS TSS (t\ ts\ ts'\ ts' = [t|ts]) TSS',
+  std.map2 MS MSS (m\ ms\ ms'\ ms' = [m|ms]) MSS'
 ].
 
 pred get-reduction-machine i:string, o:(term -> term -> term -> prop).
 get-reduction-machine "lazy" Red :- !,
   Red = t\ _\ tred\ coq.reduction.lazy.whd_all t tred.
-get-reduction-machine "cbv"  Red :- !,
-  Red = t\ _\ tred\ coq.reduction.cbv.whd_all t tred.
-get-reduction-machine "vm_compute" coq.reduction.vm.whd_all :- !.
+get-reduction-machine "compute"  Red :- !,
+  Red = t\ _\ tred\ coq.reduction.cbv.norm t tred.
+get-reduction-machine "vm_compute" coq.reduction.vm.norm :- !.
+get-reduction-machine "native_compute" coq.reduction.native.norm :- !,
+  coq.reduction.native.available?.
 
 pred parse-config i:list argument, o: list (pair string term).
 parse-config [] [] :- !.
@@ -116,30 +157,93 @@ parse-config [str Name, trm Func | ConfList] [pr Name Func | Conf] :- !,
   parse-config ConfList Conf.
 parse-config _ _ :- coq.error "ill-formed arguments".
 
-main [str RedStr, int Repeat, int Incr | ConfList] :- std.do! [
-  0 < Repeat, 0 < Incr,
-  benchmark RedStr {get-reduction-machine RedStr} {parse-config ConfList}
-            Repeat Incr 0
+main [str TimeFile, str MemFile, str RedStr, int Repeat, int Incr |
+      ConfList] :- std.do! [
+  0 < Repeat,
+  0 < Incr,
+  parse-config ConfList Config,
+  % enlarge the minor heap to 4GB
+  gc.get Minor _ _ _ _ _ _ _,
+  gc.set {calc (512 * 1024 * 1024)} _ _ _ _ _ _ _,
+  % benchmark
+  benchmark RedStr {get-reduction-machine RedStr} Config Repeat Incr 0 TSS MSS,
+  % restore the initial size of the minor heap
+  gc.set Minor _ _ _ _ _ _ _,
+  % pgfplot
+  open_out TimeFile TStream,
+  output TStream "% time consumption\n",
+  std.forall TSS (ts\ sigma Str\
+    output TStream "\\addplot coordinates {",
+    std.string.concat " " ts Str,
+    output TStream Str,
+    output TStream "};\n"),
+  output TStream "\\legend{",
+  output TStream
+    {std.string.concat ", " {std.map Config (c\ n\ sigma T\ c = pr n T)} },
+  output TStream "}\n",
+  close_out TStream,
+  open_out MemFile MStream,
+  output MStream "% memory consumption\n",
+  std.forall MSS (ms\ sigma Str\
+    output MStream "\\addplot coordinates {",
+    std.string.concat " " ms Str,
+    output MStream Str,
+    output MStream "};\n"),
+  output MStream "\\legend{",
+  output MStream
+    {std.string.concat ", " {std.map Config (c\ n\ sigma T\ c = pr n T)} },
+  output MStream "}\n",
+  close_out MStream
 ].
-main _ :- coq.error "ill-formed arguments".
+main _ :- !, coq.error "ill-formed arguments".
 
 }}.
 Elpi Typecheck.
 
-Elpi sort_benchmark
-  "lazy"       100 100
-  "sort"       (sort)
-  "CBN.sort"   (CBN.sort)
-  "CBV.sort"   (CBV.sort).
+Definition CBN_sort_lazy_bench xs :=
+  sorted N.leb (take 10 (CBN.sort N.leb xs)).
+Definition CBNOpt_sort_lazy_bench xs :=
+  sorted N.leb (take 10 (CBNOpt.sort N.leb xs)).
+Definition CBV_sort_lazy_bench xs :=
+  sorted N.leb (take 10 (CBV.sort N.leb xs)).
+Definition CBVOpt_sort_lazy_bench xs :=
+  sorted N.leb (take 10 (CBVOpt.sort N.leb xs)).
+Definition CBN_sort_bench xs    := sorted N.leb (CBN.sort N.leb xs).
+Definition CBNOpt_sort_bench xs := sorted N.leb (CBNOpt.sort N.leb xs).
+Definition CBV_sort_bench xs    := sorted N.leb (CBV.sort N.leb xs).
+Definition CBVOpt_sort_bench xs := sorted N.leb (CBVOpt.sort N.leb xs).
 
 Elpi sort_benchmark
-  "cbv"        100 100
-  "sort"       (sort)
-  "CBN.sort"   (CBN.sort)
-  "CBV.sort"   (CBV.sort).
+  "lazy1.time.out" "lazy1.mem.out" "lazy" 50 100
+  "CBN.sort"     (CBN_sort_lazy_bench)
+  "CBNOpt.sort"  (CBNOpt_sort_lazy_bench)
+  "CBV.sort"     (CBV_sort_lazy_bench)
+  "CBVOpt.sort"  (CBVOpt_sort_lazy_bench).
 
 Elpi sort_benchmark
-  "vm_compute" 100 100
-  "sort"       (sort)
-  "CBN.sort"   (CBN.sort)
-  "CBV.sort"   (CBV.sort).
+  "lazy2.time.out" "lazy2.mem.out" "lazy" 50 100
+  "CBN.sort"     (CBN_sort_bench)
+  "CBNOpt.sort"  (CBNOpt_sort_bench)
+  "CBV.sort"     (CBV_sort_bench)
+  "CBVOpt.sort"  (CBVOpt_sort_bench).
+
+Elpi sort_benchmark
+  "compute.time.out" "compute.mem.out" "compute" 50 100
+  "CBN.sort"     (CBN_sort_bench)
+  "CBNOpt.sort"  (CBNOpt_sort_bench)
+  "CBV.sort"     (CBV_sort_bench)
+  "CBVOpt.sort"  (CBVOpt_sort_bench).
+
+Elpi sort_benchmark
+  "vm.time.out" "vm.mem.out" "vm_compute" 50 1000
+  "CBN.sort"     (CBN_sort_bench)
+  "CBNOpt.sort"  (CBNOpt_sort_bench)
+  "CBV.sort"     (CBV_sort_bench)
+  "CBVOpt.sort"  (CBVOpt_sort_bench).
+
+Elpi sort_benchmark
+  "native.time.out" "native.mem.out" "native_compute" 50 1000
+  "CBN.sort"     (CBN_sort_bench)
+  "CBNOpt.sort"  (CBNOpt_sort_bench)
+  "CBV.sort"     (CBV_sort_bench)
+  "CBVOpt.sort"  (CBVOpt_sort_bench).
